examples/gcd.v
@@ -9,27 +9,28 @@ Obligation Tactic := auto.
 
 (* classical mutable Euclid's algorithm for computing GCD with subtractions *)
 
-(* two memory cells holding intermediate numbers *)
-Definition pair (p q : ptr) (x y : nat) :=
+(* two memory cells holding intermediate values *)
+Definition shape (p q : ptr) (x y : nat) :=
   [Pred h | exists h', h = p :-> x \+ (q :-> y \+ h')].
 
-(* GCD loop invariant *)
+(* GCD loop invariant: at the end both cells contain the answer *)
+(* (`unit` is needed because `Fix` always requires a single parameter) *)
 Definition gcd_loopT (p q : ptr) : Type :=
   unit ->
-  {x y : nat}, STsep (pair p q x y,
+  {x y : nat}, STsep (shape p q x y,
                      [vfun (_ : unit) h =>
-                        h \In pair p q (gcdn x y) (gcdn x y)]).
+                        h \In shape p q (gcdn x y) (gcdn x y)]).
 
 Program Definition gcd_loop (p q : ptr) :=
   Fix (fun (go : gcd_loopT p q) _ =>
-       Do (x <-- !p;
-           y <-- !q;
-           if (x : nat) != y then
-             if x < y then q ::= y - x;;
-                           go tt
-                      else p ::= x - y;;
-                           go tt
-           else ret tt)).
+    Do (x <-- !p;
+        y <-- !q;
+        if (x : nat) != y then
+          if x < y then q ::= y - x;;
+                        go tt
+                   else p ::= x - y;;
+                        go tt
+        else ret tt)).
 Next Obligation.
 (* pull out ghosts + precondition (the shape of the heap) *)
 move=>p q go _ [x [y _]] /= _ [h' ->].
@@ -37,22 +38,21 @@ move=>p q go _ [x [y _]] /= _ [h' ->].
 do 2!step; case: ltngtP=>/= [H|H|->]; step; last first.
 - (* x=y, the program is finished because GCD(y,y) = y *)
   by move=>_; rewrite gcdnn; vauto.
-- (* y<x, do the recursive call *)
+- (* y<x, do the recursive call, deconstruct the shape *)
   apply: [gE (x-y), y]=>//=; first by eauto.
-  (* the result is always successful (no exception is ever thrown) *)
-  case=>//= _ _ _ [m ->]; exists m.
+  move=>{h'} _ _ [m ->] _; exists m.
   (* use the difference property of GCD *)
-  suff: gcdn (x - y) y = gcdn x y by move=>->.
+  suff {p q go m}: gcdn (x - y) y = gcdn x y by move=>->.
   (* mathcomp's GCD theory uses addition, so we do a bit of arithmetical reasoning *)
   by rewrite gcdnC -gcdnDr gcdnC subnK //; apply: ltnW.
 (* x<y, symmetrical case to above *)
-apply: [gE x, (y-x)]=>/=; first by eauto.
-case=>//= _ _ _ [m ->]; exists m.
-suff: gcdn x (y - x) = gcdn x y by move=>->.
+apply: [gE x, (y-x)]=>//=; first by eauto.
+move=>{h'}_ _ [m ->] _; exists m.
+suff {p q go m}: gcdn x (y - x) = gcdn x y by move=>->.
 by rewrite -gcdnDr subnK //; apply: ltnW.
 Qed.
 
-(* note that there's no guarantee on termination *)
+(* note that there's no guarantee on termination, so we have only partial correctness *)
 (* i.e. the algorithm will get stuck if u = 0 /\ v != 0 or vice versa *)
 Program Definition gcd u v :
   STsep (PredT, [vfun r _ => r = gcdn u v]) :=
@@ -68,10 +68,9 @@ Program Definition gcd u v :
 Next Obligation.
 (* simplify *)
 move=>u v _ m /= _.
-(* initialize the two cells, run the loop *)
-step=>q; step=>p; apply: [stepE u, v]=>/=; first by eauto.
-(* the result is never an exception *)
-case=>//= _ _ [h' ->].
+(* initialize the two cells, run the loop, deconstruct the shape *)
+step=>q; step=>p; apply: [stepE u, v]=>//=; first by eauto.
+move=>_ _ [h' ->].
 (* run the rest of the program *)
 by do 4!step; rewrite !unitL.
 Qed.
